Tealeaves/Adapters/PolyToMono/Categorical/DecoratedMonad.v
@@ -1,0 +1,106 @@
+From Tealeaves Require Export
+  Classes.Categorical.DecoratedTraversableMonad
+  Classes.Categorical.DecoratedTraversableMonadPoly
+  Adapters.PolyToMono.Categorical.DecoratedFunctor.
+
+
+Module ToMono1.
+  Section ctx.
+
+    Context
+      {T: Type -> Type -> Type}
+      `{DecoratedMonadPoly T}.
+
+    Import DecoratedFunctor.ToMono1.
+
+    #[export] Instance Bmap_Monad_Hom:
+      forall (B1 B2: Type) (f: B1 -> B2),
+        Monad_Hom (T B1) (T B2) (fun V => @bmap T _ V B1 B2 f).
+    Proof.
+      intros.
+      constructor.
+      - typeclasses eauto.
+      - typeclasses eauto.
+      - unfold bmap.
+        unfold_ops @Map2_2.
+        typeclasses eauto.
+      - intros.
+        unfold bmap.
+        unfold_ops @Map2_2.
+        rewrite dmp_map_ret.
+        reflexivity.
+      - intros.
+        unfold bmap.
+        unfold_ops @Map2_2.
+        rewrite dmp_map_join.
+        reassociate -> on right.
+        setoid_rewrite (fun2_map2_map21 (B1 := B1) (F := T)).
+        reflexivity.
+    Qed.
+
+    #[export] Instance DecoratedMonad_PolyVar:
+      forall (B: Type), DecoratedMonad (list B) (T B).
+    Proof.
+      constructor.
+      - typeclasses eauto.
+      - typeclasses eauto.
+      - typeclasses eauto.
+      - intros.
+        unfold_ops @Decorate_PolyVar.
+        reassociate -> on left.
+        rewrite dmp_dec_ret.
+        reassociate <- on left.
+        rewrite dmp_map_ret.
+        reflexivity.
+      - intros.
+        unfold_ops @Decorate_PolyVar.
+        reassociate -> on left.
+        rewrite dmp_dec_join.
+        reassociate <- on left.
+        reassociate <- on left.
+        rewrite dmp_map_join.
+        reassociate -> near (map2 id (shift2 ∘ map_snd decp)).
+        rewrite fun2_map_map.
+        reassociate <- on right.
+        repeat reassociate -> on right.
+        repeat reassociate -> on left.
+        fequal.
+        repeat reassociate <- on right.
+        setoid_rewrite (fun2_map21_map2 (F := T)).
+        unfold shift.
+        unfold strength.
+        unfold_ops @Map2_1.
+        reassociate -> on right.
+        rewrite polydecnat.
+        reassociate <- on right.
+        setoid_rewrite (fun2_map_map (F := T)).
+        rewrite fun_map_id.
+        change (?x ∘ id) with x.
+        fequal.
+        fequal.
+        unfold shift.
+        unfold map.
+        unfold strength.
+        unfold compose.
+        ext [l t].
+        cbn.
+        compose near (decp t) on right.
+        rewrite fun2_map_map.
+        compose near (decp t) on right.
+        rewrite fun2_map_map.
+        change (?x ∘ id) with x.
+        repeat change (id ∘ ?x) with x.
+        change (id ?x) with x.
+        unfold shift2, strength2, compose.
+        compose near (decp t) on left.
+        rewrite fun2_map_map.
+        compose near (decp t) on left.
+        rewrite fun2_map_map.
+        fequal.
+        + now ext [l' b].
+        + rewrite fun_map_id.
+          reflexivity.
+    Qed.
+
+  End ctx.
+End ToMono1.
