Tealeaves/Adapters/PolyToMono/Categorical/DecoratedTraversableMonad.v
@@ -1,0 +1,5 @@
+From Tealeaves Require Export
+  Classes.Categorical.DecoratedTraversableMonad
+  Classes.Categorical.DecoratedTraversableMonadPoly.
+Adapters.PolyToMono.Categorical.Decorated
+  Adapters.PolyToMono.Categorical.DecoratedFunctor
